Splinter/Allocation.i.dfy
@@ -1,8 +1,6 @@
 // Copyright 2018-2021 VMware, Inc., Microsoft Inc., Carnegie Mellon University, ETH Zurich, and University of Washington
 // SPDX-License-Identifier: BSD-2-Clause
 
-include "Base.s.dfy"
-
 module AllocationMod {
   type AU = nat
   datatype CU = CU(au: AU, offset: nat)
