Splinter/AsyncDiskProgram.s.dfy
@@ -1,0 +1,25 @@
+// Copyright 2018-2021 VMware, Inc., Microsoft Inc., Carnegie Mellon University, ETH Zurich, and University of Washington
+// SPDX-License-Identifier: BSD-2-Clause
+
+include "Spec.s.dfy"
+include "AsyncDisk.s.dfy"
+include "../lib/Base/MapRemove.s.dfy"
+include "../lib/Checksums/CRC32C.s.dfy"
+
+// Interface to the implementer-supplied program that is getting verified.
+abstract module AsyncDiskProgram {
+  import D = AsyncDisk  // Importing for the interface, not the entire disk
+  import CrashTolerantMapSpecMod
+
+  type Variables
+  type UIOp = CrashTolerantMapSpecMod.UIOp
+
+  type DiskOp = D.DiskOp
+  type ReqRead = D.ReqRead
+  type ReqWrite = D.ReqWrite
+  type RespRead = D.RespRead
+  type RespWrite = D.RespWrite
+
+  predicate Init(s: Variables)
+  predicate Next(s: Variables, s': Variables, uiop: UIOp, dop: DiskOp)
+}
