Splinter/BetreeInterp.i.dfy
@@ -1,0 +1,141 @@
+// Copyright 2018-2021 VMware, Inc., Microsoft Inc., Carnegie Mellon University, ETH Zurich, and University of Washington
+// SPDX-License-Identifier: BSD-2-Clause
+
+include "../lib/Base/total_order.i.dfy"
+include "Tables.i.dfy"
+include "MsgSeq.i.dfy"
+include "Betree.i.dfy"
+include "Message.s.dfy"
+include "Interp.s.dfy"
+
+module BetreeInterpMod {
+  import opened Options
+  import opened MessageMod
+  import opened InterpMod
+  import opened AllocationMod
+  import opened MsgSeqMod
+  import IndirectionTableMod
+  import opened BetreeMachineMod
+  import Nat_Order
+
+  datatype LookupRecord = LookupRecord(
+    cu: CU
+  )
+  type Lookup = seq<LookupRecord>
+
+  // Select the messages that lookup finds.
+  function LookupToValue(lookup: Lookup) : Value
+    // TODO body
+
+  predicate ValidLookup(v: Variables, cache: CacheIfc.Variables, key: Key, lookup: Lookup)
+    // TODO
+
+  // What indirection table would we see if the system were running?
+  function ITbl(v: Variables, cache: CacheIfc.Variables, sb: Superblock) : Option<IndirectionTableMod.IndirectionTable> {
+    // match v {
+    //   case Starting => IndirectionTableMod.I(cache.dv /*TODO change ind tbl to expect cache*/, sb.indTbl)
+    //   case Running => Some(v.indTbl)
+    // }
+    // TODO figure out the interpretation split here
+    Some(v.indTbl)
+  }
+
+  function IMKey(v: Variables, cache: CacheIfc.Variables, sb: Superblock, key: Key) : Value
+  {
+    var indTbl := ITbl(v, cache, sb);
+    if
+      && indTbl.Some?
+      && exists lookup :: ValidLookup(v, cache, key, lookup)
+    then
+      var lookup :| ValidLookup(v, cache, key, lookup);
+      LookupToValue(lookup)
+    else
+      DefaultValue()
+  }
+
+  function IM(v: Variables, cache: CacheIfc.Variables, sb: Superblock) : (i:Interp)
+    ensures i.WF()
+  {
+    Interp(imap key | key in AllKeys() :: IMKey(v, cache, sb, key), sb.endSeq)
+  }
+
+  function IReadsKey(v: Variables, cache: CacheIfc.Variables, sb: Superblock, key: Key) : set<CU> {
+    var indTbl := ITbl(v, cache, sb);
+    if
+      && indTbl.Some?
+      && exists lookup :: ValidLookup(v, cache, key, lookup)
+    then
+      var lookup :| ValidLookup(v, cache, key, lookup);
+      set i | 0<=i<|lookup| :: var lr:LookupRecord := lookup[i]; lr.cu
+    else
+      {}
+  }
+
+  function IReadsSet(v: Variables, cache: CacheIfc.Variables, sb: Superblock) : set<CU> {
+    set cu:CU |
+      && cu in CUsInDisk()
+      && exists key :: cu in IReadsKey(v, cache, sb, key)
+  }
+
+  function IReads(v: Variables, cache: CacheIfc.Variables, sb: Superblock) : seq<CU>
+    ensures forall cu :: cu in IReads(v, cache, sb) <==> cu in IReadsSet(v, cache, sb)
+  {
+    // TODO: CU's or nats it doesn't know how to sort it. We need to fix it
+    // Nat_Order.SortSet(IReadsSet(v, cache, sb))
+    []
+  }
+
+  lemma Framing(v: Variables, cache0: CacheIfc.Variables, cache1: CacheIfc.Variables, sb:Superblock)
+    requires DiskViewsEquivalentForSet(cache0.dv, cache1.dv, IReads(v, cache0, sb))
+    ensures IM(v, cache0, sb) == IM(v, cache1, sb)
+  {
+    // TODO I'm surprised this proof passes easily.
+    // narrator: It doesn't.
+    forall key | key in AllKeys()
+      ensures IMKey(v, cache0, sb, key) == IMKey(v, cache1, sb, key)
+    {
+      var indTbl0 := ITbl(v, cache0, sb);
+      var indTbl1 := ITbl(v, cache1, sb);
+      if indTbl0.Some? && indTbl1.Some?
+      {
+        var le0 := exists lookup0 :: ValidLookup(v, cache0, key, lookup0);
+        var le1 := exists lookup1 :: ValidLookup(v, cache1, key, lookup1);
+        if le0 {
+          var lookup0 :| ValidLookup(v, cache0, key, lookup0);
+          assume ValidLookup(v, cache1, key, lookup0);
+        }
+        if le1 {
+          var lookup1 :| ValidLookup(v, cache1, key, lookup1);
+          assume ValidLookup(v, cache0, key, lookup1);
+        }
+        assert le0 == le1;
+        if (le0) {
+          // This definitely won't work.
+          var lookup0 :| ValidLookup(v, cache0, key, lookup0);
+          var lookup1 :| ValidLookup(v, cache1, key, lookup1);
+          calc {
+            IMKey(v, cache0, sb, key);
+              { assume false; } // var|
+            LookupToValue(lookup0);
+              { assume false; } // framing
+            LookupToValue(lookup1);
+              { assume false; } // var|
+            IMKey(v, cache1, sb, key);
+          }
+        } else {
+          calc {
+            IMKey(v, cache0, sb, key);
+            DefaultValue();
+            IMKey(v, cache1, sb, key);
+          }
+        }
+      }
+    }
+  }
+
+  lemma PutEffect(v: Variables, v': Variables, cache: CacheIfc.Variables, cache': CacheIfc.Variables, sb: Superblock, key: Key, value: Value, sk: Skolem)
+    ensures IM(v', cache', sb) == IM(v, cache, sb).Put(key, value)
+  {
+    assume false; // This is hard to prove -- we need to finish a tree
+  }
+}
