Splinter/Message.s.dfy
@@ -1,0 +1,21 @@
+// Copyright 2018-2021 VMware, Inc., Microsoft Inc., Carnegie Mellon University, ETH Zurich, and University of Washington
+// SPDX-License-Identifier: BSD-2-Clause
+
+include "../lib/Lang/NativeTypes.s.dfy"
+
+// TODO replace this stuff with the real key, value, message definitions
+
+module MessageMod {
+  type Key(!new,==)
+  type Value(!new)
+
+  //type Message(!new)
+  datatype Message = MessagePut(k:Key, v:Value)
+
+  function AllKeys() : iset<Key> {
+    iset key:Key | true
+  }
+
+  function DefaultValue() : Value
+    // TODO
+}
