Splinter/Spec.s.dfy
@@ -1,7 +1,8 @@
 // Copyright 2018-2021 VMware, Inc., Microsoft Inc., Carnegie Mellon University, ETH Zurich, and University of Washington
 // SPDX-License-Identifier: BSD-2-Clause
 
-include "Base.s.dfy"
+include "Message.s.dfy"
+include "Interp.s.dfy"
 include "../lib/Base/SequencesLite.s.dfy"
 
 module MapSpecMod {
